examples/cannon/CannonAll.v
@@ -8,6 +8,35 @@ Module CannonAll.
   Import inv_instances.
   Local Instance Γ : HRA := ##[invΓ; CannonAΓ].
   Local Instance Σ : GRA := ##[invΣ; Γ].
+  Local Definition irΓ : Γ := **[ir_invΓ 1; CannonAS.irΓ].
+  Local Definition irΣ : Σ := **[ir_invΣ 1; irΓ].
+
+  Local Lemma irΣ_valid : ✓ (irΣ ⋅ initial_resource_own_admin).
+  Proof.
+    eapply InitRes.app_valid.
+    { rewrite /ir_invΣ.
+      apply InitRes.app_valid.
+      { apply InitRes.singleton_some_valid, ir_ownIRA_valid. }
+      { intros i; inv_fin i. }
+    }
+    eapply InitRes.app_valid.
+    { eapply InitRes.app_valid.
+      { rewrite /ir_invΓ.
+        apply InitRes.app_valid.
+        { apply InitRes.singleton_some_valid, ir_ownERA_valid. }
+        apply InitRes.app_valid.
+        { apply InitRes.singleton_some_valid, ir_ownDRA_valid. }
+        { intros i; inv_fin i. }
+      }
+      apply InitRes.app_valid.
+      { rewrite /CannonAS.irΓ. apply InitRes.app_valid.
+        { apply InitRes.singleton_some_valid, CannonAS.ir_valid. }
+        { intros i; inv_fin i. }
+      }
+      { intros i; inv_fin i. }
+    }
+    { intros i; inv_fin i. }
+  Qed.
 
   Local Definition smod_src : SMod.t := CannonA.Mod ☆ (MainA.Mod 1).
   Local Definition spc : string → option fspec := spc_from smod_src.
@@ -56,26 +85,29 @@ Module CannonAll.
     { eapply src_tgt. }
   Qed.
 
-  Local Definition initial_resource : Σ := MainAS.init_res ⋅ CannonAS.init_res.
-  Lemma initial_resource_valid : ✓ initial_resource.
-  Proof.
-    dfs_solve.
-    apply excl_auth_valid.
-  Qed.
-
   Theorem behavioral_refinement :
     ∃ target_resource, refines_mod
-      (HMod.to_mod mod_cancel initial_resource)
+      (HMod.to_mod mod_cancel (irΣ ⋅ initial_resource_own_admin))
       (HMod.to_mod mod_tgt target_resource).
   Proof.
     move: (cancel_tgt)=>H; rewrite /refines in H; des; ss.
-    destruct (H initial_resource).
-    { apply initial_resource_valid. }
-    { iIntros "I"; rewrite /init_cond /CannonA.init_cond /MainA.init_cond.
-      rewrite /precond /= /CannonAS.Ready /CannonAS.Ball
-        own.Own_eq own.own_eq /own.Own_def /own.own_def.
-      rewrite /initial_resource /MainAS.init_res /CannonAS.init_res. Set Printing Implicit.
-      iDestruct "I" as "[I1 I2]"; iFrame. iSplit; iPureIntro; ss.
+    destruct (H (irΣ ⋅ initial_resource_own_admin)).
+    { apply irΣ_valid. }
+    { rewrite /irΣ /InitRes.app.
+      try (repeat rewrite ?InitRes.L_distr ?InitRes.R_distr).
+      iIntros "[[[I _] [[[E [D _]] [[M _] _]] _]] O]".
+      iPoseProof (make_wsats 1 with "[I E D]") as "[U W]".
+      { iSplitL "I".
+        { solve_index "I". f_equal. }
+        iSplitL "E".
+        { solve_index "E". f_equal. }
+        { solve_index "D". f_equal. }
+      }
+      iPoseProof (CannonAS.ReadyBall with "[M]") as "[R B]".
+      { rewrite /CannonAS.Fired. solve_index "M". f_equal. }
+      iSplitL "R".
+      { rewrite /init_cond. iFrame. }
+      unfold_pre_post. iFrame. iSplit; eauto.
     }
     { econs; ss; try prove_nodup. }
     { exists x; des; eauto. }
