examples/spinlock/SpinLockAll.v
@@ -5,253 +5,6 @@ Require Import SpinLockMainHeader SpinLockMainI SpinLockMainA SpinLockMainIAProo
 Require Import SchHeader SchI SchA SchIAproof.
 Require Import ElimRel SModCancel Cancellation.
 
-Ltac gen_eq a :=
-  match a with context [?t] =>
-    lazymatch t with
-    | eq_refl => fail
-    | _ =>
-      let T := type of t in
-      match (eval simpl in T) with
-      | _ = _ => generalize t
-      end
-    end
-  end.
-
-Ltac gen_prop a :=
-  match a with context [?t] =>
-    let T := type of t in
-    match (eval simpl in T) with
-    | Prop => generalize t
-    end
-  end.
-
-Ltac remove_eq_aux :=
-  let e := fresh "E" in
-  intros e;
-  match goal with
-  | H : @eq ?A ?b _ |- _ => replace H with (@eq_refl A b)
-  end; last apply UIP; clear e.
-
-Ltac remove_eq a := gen_eq a; remove_eq_aux.
-
-From iris Require Import csum.
-
-Module InitRes.
-  Definition nil : GRAs.nil.
-  Proof. intros i; inv i. Defined.
-
-  Definition singleton {A : DRA} (a : option A) : GRAs.singleton A.
-  Proof.
-    intros i γ. inv_fin i.
-    { destruct (decide (γ = base_γ)).
-      { destruct a as [a|].
-        { ss. exact (Some (Cinr a)). }
-        { ss. exact (Some (Cinl (Excl ()))). }
-      }
-      { exact None. }
-    }
-    { intros i. inv i. }
-  Defined.
-
-  Definition R_prf {Σ1 Σ2 : GRA} (i2 : gid Σ2) :
-    @eq cmra
-    (allocs.allocsUR positive (@GRA_lookup Σ2 i2))
-    (allocs.allocsUR positive (@GRA_lookup (GRAs.app Σ1 Σ2) (Fin.R (@GRA_len Σ1) i2))).
-  Proof. rewrite /GRAs.app /= fin_add_inv_r; refl. Qed.
-
-  Definition L_prf {Σ1 Σ2 : GRA} (i1 : gid Σ1) :
-    @eq cmra
-    (allocs.allocsUR positive (@GRA_lookup Σ1 i1))
-    (allocs.allocsUR positive (@GRA_lookup (GRAs.app Σ1 Σ2) (Fin.L (@GRA_len Σ2) i1))).
-  Proof. rewrite /GRAs.app /= fin_add_inv_l; refl. Qed.
-
-  Definition R {Σ1 Σ2 : GRA} (r2 : Σ2) : GRAs.app Σ1 Σ2.
-  Proof.
-    intros i. eapply fin_add_inv with (i:=i).
-    { intros i1 g. exact ε. }
-    { intros i2. refine (cmra_transport (R_prf i2) (r2 i2)). }
-  Defined.
-
-  Definition L {Σ1 Σ2 : GRA} (r1 : Σ1) : GRAs.app Σ1 Σ2.
-  Proof.
-    intros i. eapply fin_add_inv with (i:=i).
-    { intros i1. refine (cmra_transport (L_prf i1) (r1 i1)). }
-    { intros i2 g. exact ε. }
-  Defined.
-
-  Lemma R_distr {Σ1 Σ2 : GRA} (r1 r2 : Σ2) : @R Σ1 Σ2 (r1 ⋅ r2) = @R Σ1 Σ2 r1 ⋅ @R Σ1 Σ2 r2.
-  Proof.
-    extensionalities i; apply fin_add_inv with (i:=i); clear i.
-    { intros i1; rewrite /R ?discrete_fun_lookup_op ?fin_add_inv_l //. }
-    { intros i2. rewrite /R discrete_fun_lookup_op fin_add_inv_r.
-      rewrite !fin_add_inv_r cmra_transport_op //.
-    }
-  Qed.
-
-  Lemma L_distr {Σ1 Σ2 : GRA} (r1 r2 : Σ1) : @L Σ1 Σ2 (r1 ⋅ r2) = @L Σ1 Σ2 r1 ⋅ @L Σ1 Σ2 r2.
-  Proof.
-    extensionalities i; apply fin_add_inv with (i:=i); clear i.
-    { intros i1. rewrite /L discrete_fun_lookup_op fin_add_inv_l.
-      rewrite !fin_add_inv_l cmra_transport_op //.
-    }
-    { intros i2; rewrite /L ?discrete_fun_lookup_op ?fin_add_inv_r //. }
-  Qed.
-
-  Definition app {Σ1 Σ2 : GRA} (r1 : Σ1) (r2 : Σ2) : GRAs.app Σ1 Σ2 :=
-    @L Σ1 Σ2 r1 ⋅ @R Σ1 Σ2 r2.
-
-  Lemma singleton_some_valid {A : DRA} (a : A)
-      (VALID : ✓ a) :
-    ✓ (singleton (Some a) ⋅ initial_resource_own_admin).
-  Proof.
-    intros i γ. inv_fin i; ss; des_ifs.
-    { rewrite ?discrete_fun_lookup_op /singleton /initial_resource_own_admin.
-      des_ifs. ss. rewrite left_id /allocs.allocs_auth; des_ifs; ss.
-    }
-    { intros i; inv i. }
-  Qed.
-
-  Lemma singleton_none_valid {A : DRA} :
-    ✓ (@singleton A None ⋅ initial_resource_own_admin).
-  Proof.
-    intros i γ. inv_fin i; ss; des_ifs.
-    { rewrite ?discrete_fun_lookup_op /singleton /initial_resource_own_admin.
-      des_ifs; ss; rewrite left_id /allocs.allocs_auth; des_ifs.
-    }
-    { intros i; inv i. }
-  Qed.
-
-  Definition app_valid {Σ1 Σ2 : GRA} (r1 : Σ1) (r2 : Σ2)
-      (VALID1 : ✓ (r1 ⋅ initial_resource_own_admin))
-      (VALID2 : ✓ (r2 ⋅ initial_resource_own_admin)) :
-    ✓ (app r1 r2 ⋅ initial_resource_own_admin).
-  Proof.
-    intros i; apply fin_add_inv with (i:=i).
-    { intros i1. rewrite /app ?discrete_fun_lookup_op.
-      rewrite /L fin_add_inv_l /R fin_add_inv_l right_id.
-      rewrite /initial_resource_own_admin.
-      match goal with | |- ?A => gen_eq A end.
-      rewrite /GRAs.app /= fin_add_inv_l. remove_eq_aux. ss.
-    }
-    { intros i2. rewrite /app ?discrete_fun_lookup_op.
-      rewrite /L fin_add_inv_r /R fin_add_inv_r left_id.
-      rewrite /initial_resource_own_admin.
-      match goal with | |- ?A => gen_eq A end.
-      rewrite /GRAs.app /= fin_add_inv_r. remove_eq_aux. ss.
-    }
-  Qed.
-
-  Lemma singleton_index {A : DRA} (a : A) :
-    singleton (Some a) = discrete_fun_singleton 0%fin (allocs.allocs_frag base_γ a).
-  Proof.
-    extensionalities i g. inv_fin i; ss; des_ifs.
-    { rewrite ?discrete_fun_lookup_singleton //=. }
-    { rewrite discrete_fun_lookup_singleton /= /allocs.allocs_frag discrete_fun_lookup_singleton_ne //. }
-    { intros i; inv i. }
-  Qed.
-
-  Lemma L_index {Σ1 Σ2 : GRA} (i : fin (@GRA_len Σ1)) r :
-    @L Σ1 Σ2 (discrete_fun_singleton i r)
-    = discrete_fun_singleton (Fin.L (@GRA_len Σ2) i) (cmra_transport (@L_prf Σ1 Σ2 i) r).
-  Proof.
-    rewrite /L. extensionalities i1.
-    apply fin_add_inv with (i:=i1); cycle 1.
-    { intros i2; ss.
-      match goal with | |- fin_add_inv ?P ?H1 ?H2 ?r = _ => rewrite (fin_add_inv_r P H1 H2 _) end.
-      rewrite discrete_fun_lookup_singleton_ne; ss.
-      ii. eapply Fin.L_R_neq; eauto.
-    }
-    { intros i2; ss.
-      destruct (decide (i = i2)).
-      { subst.
-        match goal with | |- fin_add_inv ?P ?H1 ?H2 ?r = _ => rewrite (fin_add_inv_l P H1 H2 _) end.
-        rewrite ?discrete_fun_lookup_singleton //.
-      }
-      { match goal with | |- fin_add_inv ?P ?H1 ?H2 ?r = _ => rewrite (fin_add_inv_l P H1 H2 _) end.
-        rewrite ?discrete_fun_lookup_singleton_ne //.
-        { match goal with | |- ?a => gen_eq a end.
-          rewrite /GRAs.app /= fin_add_inv_l. remove_eq_aux. ss.
-        }
-        { ii. apply Fin.L_inj in H. ss. }
-      }
-    }
-  Qed.
-
-  Lemma R_index {Σ1 Σ2 : GRA} (i : fin (@GRA_len Σ2)) r :
-    @R Σ1 Σ2 (discrete_fun_singleton i r)
-    = discrete_fun_singleton (Fin.R (@GRA_len Σ1) i) (cmra_transport (@R_prf Σ1 Σ2 i) r).
-  Proof.
-    rewrite /R. extensionalities i1.
-    apply fin_add_inv with (i:=i1); cycle 1.
-    { intros i2; ss.
-      match goal with | |- fin_add_inv ?P ?H1 ?H2 ?r = _ => rewrite (fin_add_inv_r P H1 H2 _) end.
-      destruct (decide (i = i2)).
-      { subst. rewrite ?discrete_fun_lookup_singleton //.
-      }
-      { rewrite ?discrete_fun_lookup_singleton_ne //.
-        { match goal with | |- ?a => gen_eq a end.
-          rewrite /GRAs.app /= fin_add_inv_r. remove_eq_aux. ss.
-        }
-        { ii. apply Fin.R_inj in H. ss. }
-      }
-    }
-    { intros i2; ss.
-      match goal with | |- fin_add_inv ?P ?H1 ?H2 ?r = _ => rewrite (fin_add_inv_l P H1 H2 _) end.
-      rewrite discrete_fun_lookup_singleton_ne; ss.
-      ii. eapply Fin.L_R_neq; eauto.
-    }
-  Qed.
-End InitRes.
-Notation "*[ ]" := InitRes.nil (format "*[ ]").
-Notation "*[ Σ1 ; .. ; Σn ]" :=
-  (InitRes.app (InitRes.singleton Σ1) .. (InitRes.app (InitRes.singleton Σn) InitRes.nil) ..).
-Notation "**[ Σ1 ; .. ; Σn ]" := (InitRes.app Σ1 .. (InitRes.app Σn InitRes.nil) ..).
-
-Ltac unfold_own :=
-  match goal with
-  | |- Own ?R = own base_γ ?R2 =>
-    rewrite own.Own_eq /own.Own_def own.own_eq /own.own_def /own.iRes_singleton; f_equal
-  end.
-
-Ltac unfold_left :=
-  repeat match goal with
-  | |- context [InitRes.singleton _] => rewrite InitRes.singleton_index
-  | |- context [InitRes.L (discrete_fun_singleton _ _)] => rewrite ?InitRes.L_index
-  | |- context [InitRes.R (discrete_fun_singleton _ _)] => rewrite ?InitRes.R_index
-  end.
-
-Hint Unfold invG_I invG_Σ invG_subG subG_invΣ subG_inG : GRA_index.
-Hint Unfold sProp.in_subG_obligation_1 in_subG invG_E invG_Γ subG_invΓ invG_D : GRA_index.
-
-Ltac solve_index H := 
-  eapply eq_ind; first iExact H;
-  unfold_own;
-  etrans;
-  [unfold_left; repeat match goal with | |- ?a = _ => remove_eq a end; simpl; refl
-  | etrans; cycle 1;
-    [ symmetry;
-      let k := fresh "k" in
-      match goal with
-      | |- context [inG_id ?i] => pattern i; match goal with | |- ?f ?a => set (k:=f) end
-      end;
-      autounfold with GRA_index
-      ; subst k
-      ; simpl
-      ; hrepeat do 1 match goal with | |- ?a = _ => remove_eq a end
-      ; simpl
-    | refl
-    ]
-  ].
-
-Lemma ir_own_admin {Σ : GRA} : Own initial_resource_own_admin ⊢ own_admin.
-Proof.
-  rewrite own.own_admin_eq /own.own_admin_def.
-  iIntros "H". iExists (⊤ ∖ {[base_γ]}).
-  iSplit.
-  { iPureIntro. eapply difference_infinite, singleton_finite. eapply top_infinite. }
-  { rewrite /initial_resource_own_admin own.Own_eq /own.Own_def. iFrame. }
-Qed.
-
 Module SpinLockAll.
   Import inv_instances.
   Local Definition u : univ_id := 1.
@@ -260,76 +13,43 @@ Module SpinLockAll.
   Local Definition genv : GEnv.t := GEnv.unit.
 
   Local Instance Γ : HRA := ##[invΓ; memΓ; SchAΓ; SpinLockΓ; SpinLockMainAΓ].
-
-  Definition IRownIRA : DRA_mk ownIRA :=
-    ownI_initial u.
-  Lemma IRownIRA_valid : ✓ (IRownIRA). eapply (ownI_initial_valid u). Qed.
-
   Local Instance Σ : GRA := ##[invΣ; SchAΣ; Γ].
 
-  Definition IRownDRA : DRA_mk ownDRA :=
-    ownD_initial u.
-  Lemma IRownDRA_valid : ✓ (IRownDRA). eapply ownD_initial_valid. Qed.
+  Definition irΓ : Γ :=
+    **[ir_invΓ u; ir_memΓ csl genv; SchAS.ir_SchAΓ; *[None]; *[None]].
+  Definition irΣ : Σ :=
+    **[ir_invΣ u; SchAS.ir_SchAΣ; irΓ].
 
-  Definition IRownERA : DRA_mk ownERA :=
-    ownE_initial u.
-  Lemma IRownERA_valid : ✓ (IRownERA). eapply ownE_initial_valid. Qed.
-
-  Definition IRmemRA : DRA_mk memRA :=
-    mem_initial_mem_r csl genv.
-  Lemma IRmemRA_valid : ✓ (IRmemRA).
-  Proof. pose proof (mem_initial_valid csl genv). rewrite /IRmemRA. eapply cmra_valid_op_l; eauto. Qed.
-
-  Definition IRthreadsRA : DRA_mk threadsRA :=
-    SchAS.threadsRA_initial.
-  Lemma IRthreadsRA_valid : ✓ (IRthreadsRA). apply SchAS.threadsRA_initial_valid. Qed.
-
-  Definition IRtidRA : DRA_mk tidRA :=
-    SchAS.tidRA_initial.
-  Lemma IRtidRA_valid : ✓ (IRtidRA). apply SchAS.tidRA_initial_valid. Qed.
-
-  Definition IRinvΓ : invΓ :=
-    *[Some (IRownERA); Some (IRownDRA)].
-  Definition IRmemΓ : memΓ :=
-    *[Some IRmemRA].
-  Definition IRSchAΓ : SchAΓ :=
-    *[Some IRtidRA].
-
-  Definition IRΓ : Γ :=
-    **[IRinvΓ; IRmemΓ; IRSchAΓ; *[None]; *[None]].
-
-  Definition IRΣ : Σ :=
-    **[*[Some (IRownIRA)]; *[Some IRthreadsRA]; IRΓ].
-
-  Lemma IRΣ_valid : ✓ (IRΣ ⋅ initial_resource_own_admin).
+  Lemma irΣ_valid : ✓ (irΣ ⋅ initial_resource_own_admin).
   Proof.
     eapply InitRes.app_valid.
-    { apply InitRes.app_valid.
-      { apply InitRes.singleton_some_valid, IRownIRA_valid. }
+    { rewrite /ir_invΣ.
+      apply InitRes.app_valid.
+      { apply InitRes.singleton_some_valid, ir_ownIRA_valid. }
       { intros i; inv_fin i. }
     }
     apply InitRes.app_valid.
     { apply InitRes.app_valid.
-      { apply InitRes.singleton_some_valid, IRthreadsRA_valid. }
+      { apply InitRes.singleton_some_valid, SchAS.ir_threadsRA_valid. }
       { intros i; inv_fin i. }
     }
     apply InitRes.app_valid.
     { apply InitRes.app_valid.
-      { apply InitRes.app_valid.
-        { apply InitRes.singleton_some_valid, IRownERA_valid. }
+      { rewrite /ir_invΓ. apply InitRes.app_valid.
+        { apply InitRes.singleton_some_valid, ir_ownERA_valid. }
         { apply InitRes.app_valid.
-          { apply InitRes.singleton_some_valid, IRownDRA_valid. }
+          { apply InitRes.singleton_some_valid, ir_ownDRA_valid. }
           { intros i; inv_fin i. }
         }
       }
       apply InitRes.app_valid.
-      { apply InitRes.app_valid.
-        { apply InitRes.singleton_some_valid, IRmemRA_valid. }
+      { rewrite /ir_memΓ. apply InitRes.app_valid.
+        { apply InitRes.singleton_some_valid, ir_memRA_valid. }
         { intros i; inv_fin i. }
       }
       apply InitRes.app_valid.
       { apply InitRes.app_valid.
-        { apply InitRes.singleton_some_valid, IRtidRA_valid. }
+        { apply InitRes.singleton_some_valid, SchAS.ir_tidRA_valid. }
         { intros i; inv_fin i. }
       }
       apply InitRes.app_valid.
@@ -352,19 +72,39 @@ Module SpinLockAll.
 
   (* building the source module *)
   Local Definition spc_user_s : string → option fspec :=
-    to_spc (SpinLockMainAS.spc u ++ MemA.Spc ++ SpinLockAS.spc u).
-
+    to_spc (SpinLockMainAS.spc u ++ MemA.spc ++ SpinLockAS.spc u).
   Local Definition smod_src : SMod.t :=
     SpinLockMainA.Mod u ☆ MemA.Mod ☆ SchA.Mod u spc_user_s ☆ SpinLockA.Mod u.
   Local Definition spc_s : string → option fspec :=
     spc_from smod_src.
   Local Definition mod_src : HMod.t := SMod.to_hmod (wsim_ginv u ⊤) spc_s smod_src.
-  Local Definition init_cond : iProp Σ := (MemA.InitCond csl genv ∗ SchA.InitCond)%I.
-  Definition a : invG α Σ Γ. apply _. Defined.
+  Local Definition init_cond : iProp Σ := (MemA.init_cond csl genv ∗ SchA.init_cond)%I.
 
   (* source module after cancellation *)
   Local Definition smod_cancel : HMod.t := SModCancel.to_hmod smod_src.
 
+  (* Some assumptions on spc inclusion *)
+  Lemma SchInSpc : spc_incl (SchAS.spc u spc_user_s) spc_s.
+  Proof.
+    rewrite /spc_user_s /SchAS.spc /spc_s /smod_src; unseal CRIS. split; first prove_nodup.
+    ii. ss; des_ifs; rewrite ->eq_rel_dec_correct in *; des_ifs.
+  Qed.
+  Lemma MainInSpc : spc_incl (SpinLockMainAS.spc u) spc_user_s.
+  Proof.
+    rewrite /spc_user_s /SpinLockMainAS.spc /spc_s /smod_src; unseal CRIS. split; first prove_nodup.
+    ii. ss; des_ifs; rewrite ->eq_rel_dec_correct in *; des_ifs.
+  Qed.
+  Lemma MemInSpc : spc_incl (MemA.spc) spc_s.
+  Proof.
+    rewrite /spc_user_s /MemA.spc /spc_s /smod_src; unseal CRIS. split; first prove_nodup.
+    ii. ss; des_ifs; rewrite ->eq_rel_dec_correct in *; des_ifs.
+  Qed.
+  Lemma UserInSpc : spc_sub spc_user_s spc_s.
+  Proof.
+    rewrite /spc_user_s /spc_s /MemA.spc; unseal CRIS.
+    ii; ss; des_ifs; rewrite ->eq_rel_dec_correct in *; des_ifs.
+  Qed.
+    
   (* Refinement between smod_cancel and smod_src *)
   Local Definition main_fsp : fspec := SpinLockMainAS.main_spec u.
   Lemma cancel_src :
@@ -391,16 +131,9 @@ Module SpinLockAll.
       rewrite hmod_add_assoc -hmod_addc_empty_l.
       etrans; first eapply ctxr_cond_frameR.
       { eapply SpinLockMainIA.wctxr; eauto.
-        { instantiate (1:=spc_user_s).
-          rewrite /spc_user_s /SchAS.spc /spc_s /smod_src; unseal CRIS. split; first prove_nodup.
-          ii. ss; des_ifs; rewrite ->eq_rel_dec_correct in *; des_ifs.
-        }
-        { rewrite /spc_user_s /SchAS.spc /spc_s /smod_src; unseal CRIS. split; first prove_nodup.
-          ii. ss; des_ifs; rewrite ->eq_rel_dec_correct in *; des_ifs.
-        }
-        { rewrite /spc_user_s /MemA.Spc /spc_s /smod_src; unseal CRIS. split; first prove_nodup.
-          ii. ss; des_ifs; rewrite ->eq_rel_dec_correct in *; des_ifs.
-        }
+        { apply SchInSpc. }
+        { apply MainInSpc. }
+        { apply MemInSpc. }
       }
       rewrite hmod_addc_empty_l. refl.
     }
@@ -409,19 +142,14 @@ Module SpinLockAll.
     { eapply ctxr_frameR. rewrite -hmod_addc_empty_l. eapply ctxr_cond_frameR.
       etrans; first eapply ctxr_comm.
       eapply SpinLockIA.wctxr.
-      { rewrite /spc_user_s /SchAS.spc /spc_s /smod_src; unseal CRIS. split; first prove_nodup.
-        ii. ss; des_ifs; rewrite ->eq_rel_dec_correct in *; des_ifs.
-      }
-      { rewrite /spc_user_s /spc_s /smod_src /MemA.Spc; unseal CRIS. split; first prove_nodup.
-        ii. ss; des_ifs; rewrite ->eq_rel_dec_correct in *; des_ifs.
-      }
+      { apply SchInSpc. }
+      { apply MemInSpc. }
     }
     rewrite hmod_add_assoc.
     etrans; first eapply ctxr_comm. rewrite -hmod_add_assoc. eapply ctxr_frameR.
     etrans.
     { rewrite hmod_addc_empty_l. eapply ctxr_frameR, ctxr_cond_frameR. eapply MemIA.wctxr.
-      rewrite /MemA.Spc; unseal CRIS.
-      split; first prove_nodup. ii; ss; des_ifs; rewrite ->eq_rel_dec_correct in *; des_ifs.
+      apply MemInSpc.
     }
     eapply ctxr_frameL.
     etrans.
@@ -429,12 +157,8 @@ Module SpinLockAll.
       { unfold_hmod; ss. }
       rewrite hmod_addc_empty_l.
       eapply SchIA.wctxr.
-      { rewrite /spc_user_s /SchAS.spc /spc_s /smod_src; unseal CRIS. split; first prove_nodup.
-        ii. ss; des_ifs; rewrite ->eq_rel_dec_correct in *; des_ifs.
-      }
-      { rewrite /spc_user_s /SchAS.spc /spc_s /smod_src /MemA.Spc; unseal CRIS.
-        ii. ss; des_ifs; rewrite ->eq_rel_dec_correct in *; des_ifs.
-      }
+      { apply SchInSpc. }
+      { apply UserInSpc. }
     }
     refl.
   Qed.
@@ -448,23 +172,18 @@ Module SpinLockAll.
     { eapply src_tgt. }
   Qed.
 
-  Notation "'L'" := InitRes.L (at level 50, only printing).
-  Notation "'R'" := InitRes.R (at level 50, only printing).
-
-  Hint Unfold SchA.RA_inG SchA.RA_inG0 SchA.subG_GΣ SchA.subG_GΓ : GRA_index.
-
   Theorem behavioral_refinement :
     ∃ target_resource, refines_mod
-      (HMod.to_mod smod_cancel (IRΣ ⋅ initial_resource_own_admin))
+      (HMod.to_mod smod_cancel (irΣ ⋅ initial_resource_own_admin))
       (HMod.to_mod mod_tgt target_resource).
   Proof.
     move: (cancel_tgt)=>H; rewrite /refines in H; ss.
-    destruct (H ((IRΣ ⋅ initial_resource_own_admin))).
-    { apply IRΣ_valid. }
-    { rewrite /IRΣ /InitRes.app.
+    destruct (H ((irΣ ⋅ initial_resource_own_admin))).
+    { apply irΣ_valid. }
+    { rewrite /irΣ /InitRes.app.
       try (repeat rewrite ?InitRes.L_distr ?InitRes.R_distr).
       iIntros "[[[I _] [[THS _] [[[E [D _]] [[M _] [[TID _] _]]] _]]] O]".
-      iPoseProof (ownI_initial_gen u with "[I E D]") as "[U W]".
+      iPoseProof (make_wsats u with "[I E D]") as "[U W]".
       { iSplitL "I".
         { solve_index "I". f_equal. }
         iSplitL "E".
@@ -475,13 +194,13 @@ Module SpinLockAll.
       { rewrite /SchAS.tid_admin. unseal "SchA". solve_index "TID". f_equal. }
       iPoseProof (SchAS.tid_admin_none_split 0 with "TID") as "[H1 H2]".
       { iSplitR "U W O H2"; cycle 1.
-        { iPoseProof (ir_own_admin with "O") as "$". unfold_pre_post; iFrame. iSplit; eauto. }
+        { iPoseProof (make_own_admin with "O") as "$". unfold_pre_post; iFrame. iSplit; eauto. }
         rewrite /init_cond. iSplitL "M".
-        { rewrite /MemA.InitCond /mem_initial_mem. solve_index "M". f_equal. }
-        iSplitL "THS".
-        { rewrite /SchAS.initial_threads. unseal "SchA". rewrite /IRthreadsRA /SchAS.threadsRA_initial.
-          solve_index "THS". f_equal.
+        { iAssert (mem_init csl genv) with "[M]" as "[$ _]".
+          { rewrite /mem_init. solve_index "M". f_equal. }
         }
+        iSplitL "THS".
+        { rewrite /SchAS.init_threads. unseal "SchA". solve_index "THS". f_equal. }
         { iFrame. }
       }
     }
